cleanq/crb: update the hoare triples and first step of general cleanup
Signed-off-by: Reto Achermann <reto.achermann@inf.ethz.ch>

CleanQ/CleanQ_CRBModel.thy
@@ -286,17 +286,35 @@ text \<open>
 subsubsection \<open>Enqueue Operation\<close>
 (* ------------------------------------------------------------------------------------ *)
 
+text \<open>
+  The first part of the \verb+enqueue+ operation is to write head buffer element into
+  the ring at the head position.
+\<close>
+
 definition CleanQ_RB_write_head_x :: "'a \<Rightarrow> 'a CleanQ_RB_State \<Rightarrow> 'a CleanQ_RB_State" 
   where "CleanQ_RB_write_head_x b rb = rb \<lparr>rTXY := rb_write_head b (rTXY rb) \<rparr>"
-
-definition CleanQ_RB_incr_head_x :: "'a \<Rightarrow> 'a CleanQ_RB_State \<Rightarrow> 'a CleanQ_RB_State" 
-  where "CleanQ_RB_incr_head_x b rb = rb \<lparr>rTXY := rb_incr_head (rTXY rb), rSX := (rSX rb) - {b} \<rparr>"
 
 definition CleanQ_RB_write_head_y :: "'a \<Rightarrow> 'a CleanQ_RB_State \<Rightarrow> 'a CleanQ_RB_State" 
   where "CleanQ_RB_write_head_y b rb = rb \<lparr>rTYX := rb_write_head b (rTYX rb) \<rparr>"
 
+text \<open>
+  The second part is to increment the head pointer, this effectively transfers the 
+  ownership of the buffer from the owning sets SX or SY to the transfer set TXY or TYX. 
+\<close>
+
+definition CleanQ_RB_incr_head_x :: "'a \<Rightarrow> 'a CleanQ_RB_State \<Rightarrow> 'a CleanQ_RB_State" 
+  where "CleanQ_RB_incr_head_x b rb = rb \<lparr>rTXY := rb_incr_head (rTXY rb), 
+                                          rSX := (rSX rb) - {b} \<rparr>"
+
 definition CleanQ_RB_incr_head_y :: "'a \<Rightarrow> 'a CleanQ_RB_State \<Rightarrow> 'a CleanQ_RB_State" 
-  where "CleanQ_RB_incr_head_y b rb = rb \<lparr>rTYX := rb_incr_head (rTYX rb), rSY := (rSY rb) - {b} \<rparr>"
+  where "CleanQ_RB_incr_head_y b rb = rb \<lparr> rTYX := rb_incr_head (rTYX rb), 
+                                           rSY := (rSY rb) - {b} \<rparr>"
+
+
+text \<open>
+  We define helper functions to read the head pointer of the ring buffer and to check
+  whether the head position of the ring is \verb+None+ or it contains some buffer.
+\<close>
 
 definition CleanQ_RB_read_head_x :: "'a CleanQ_RB_State \<Rightarrow> 'a " 
   where "CleanQ_RB_read_head_x rb = rb_read_head (rTXY rb)"
@@ -310,222 +328,10 @@ definition CleanQ_RB_head_none_x :: "'a CleanQ_RB_State \<Rightarrow> bool"
 definition CleanQ_RB_head_none_y :: "'a CleanQ_RB_State \<Rightarrow> bool" 
   where "CleanQ_RB_head_none_y rb = rb_head_none (rTYX rb)"
 
-lemma CleanQ_split_enq_x_equal[simp]:
-  shows "CleanQ_RB_incr_head_x b (CleanQ_RB_write_head_x b rb) = CleanQ_RB_enq_x b rb"
-  unfolding CleanQ_RB_incr_head_x_def CleanQ_RB_write_head_x_def CleanQ_RB_enq_x_def
-  rb_enq_def by simp
 
-lemma CleanQ_split_enq_y_equal[simp]:
-  shows "CleanQ_RB_incr_head_y b (CleanQ_RB_write_head_y b rb) = CleanQ_RB_enq_y b rb"
-  unfolding CleanQ_RB_incr_head_y_def CleanQ_RB_write_head_y_def CleanQ_RB_enq_y_def
-  rb_enq_def by simp
-
-
-text \<open>
-  The two operations \verb+CleanQ_RB_enq_x+ and \verb+CleanQ_RB_enq_y+ as partial 
-  operations also preserver the invariants. To show this we need some helper lemmas.
-  First writeing at head does not invalidate the Invariants since it is the same
-  state from the invariants persective as withouth the write. 
+text \<open> 
+  Writing the head location in the ring ensures that the head is not none. 
 \<close>
-
-lemma CleanQ_RB_enq_x_write_list:
-  assumes Inv:" CleanQ_RB_Invariants K rb" and
-          sx: "b \<in> rSX rb" and
-          enq:"CleanQ_RB_enq_x_possible rb" 
-  shows "CleanQ_RB_list (rTXY (CleanQ_RB_write_head_x b rb)) = CleanQ_RB_list (rTXY rb)"
-  using assms
-  by (metis CleanQ_RB_State.select_convs(3) CleanQ_RB_State.surjective CleanQ_RB_State.update_convs(3) 
-      CleanQ_RB_write_head_x_def rb_enq_write_same) 
-
-lemma CleanQ_RB_enq_y_write_list:
-  assumes Inv:" CleanQ_RB_Invariants K rb" and
-          sy: "b \<in> rSY rb" and
-          enq:"CleanQ_RB_enq_y_possible rb" 
-  shows "CleanQ_RB_list (rTYX (CleanQ_RB_write_head_y b rb)) = CleanQ_RB_list (rTYX rb)"
-  using assms
-  by (metis CleanQ_RB_State.ext_inject CleanQ_RB_State.surjective CleanQ_RB_State.update_convs(4) CleanQ_RB_write_head_y_def rb_enq_write_same)
-
-lemma CleanQ_RB_enq_x_write_can_enq:
-  assumes Inv:" CleanQ_RB_Invariants K rb" and
-          sx: "b \<in> rSX rb" and
-          enq:"CleanQ_RB_enq_x_possible rb" 
-  shows "CleanQ_RB_enq_x_possible (CleanQ_RB_write_head_x b rb)"
-  using assms
-  by (simp add: CleanQ_RB_write_head_x_def CleanQ_RB_enq_x_possible_def 
-      rb_enq_write_can_enq) 
-
-lemma CleanQ_RB_enq_y_write_can_enq:
-  assumes Inv:" CleanQ_RB_Invariants K rb" and
-          sx: "b \<in> rSY rb" and
-          enq:"CleanQ_RB_enq_y_possible rb" 
-  shows "CleanQ_RB_enq_y_possible (CleanQ_RB_write_head_y b rb)"
-  using assms
-  by (simp add: CleanQ_RB_write_head_y_def CleanQ_RB_enq_y_possible_def 
-      rb_enq_write_can_enq) 
-
-
-lemma CleanQ_RB_write_head_y_can_enq_x:
-  "CleanQ_RB_Invariants K rb \<Longrightarrow> 
-   CleanQ_RB_enq_x_possible rb = CleanQ_RB_enq_x_possible (CleanQ_RB_write_head_y b rb)"
-  by (simp add: CleanQ_RB_write_head_y_def CleanQ_RB_enq_x_possible_def) 
-
-lemma CleanQ_RB_write_head_y_can_deq_x:
-"CleanQ_RB_Invariants K rb \<Longrightarrow> 
-  CleanQ_RB_deq_x_possible rb = CleanQ_RB_deq_x_possible (CleanQ_RB_write_head_y b rb)"
-  by(simp add: CleanQ_RB_deq_x_possible_def CleanQ_RB_write_head_y_def rb_write_can_deq)
-
-lemma CleanQ_RB_write_head_y_can_deq_y:
-  "CleanQ_RB_Invariants K rb \<Longrightarrow> 
-  CleanQ_RB_deq_y_possible rb = CleanQ_RB_deq_y_possible (CleanQ_RB_write_head_y b rb)"
-  by (simp add: CleanQ_RB_deq_y_possible_def CleanQ_RB_write_head_y_def)
-
-lemma CleanQ_RB_write_head_y_can_enq_y:
-"CleanQ_RB_Invariants K rb \<Longrightarrow> 
-  CleanQ_RB_enq_y_possible rb = CleanQ_RB_enq_y_possible (CleanQ_RB_write_head_y b rb)"
-  by(simp add: CleanQ_RB_enq_y_possible_def CleanQ_RB_write_head_y_def rb_write_can_enq)
-   
-
-lemmas CleanQ_RB_write_head_y_can_enq_deq_simps  = CleanQ_RB_write_head_y_can_enq_x 
-                                                  CleanQ_RB_write_head_y_can_deq_x 
-                                                  CleanQ_RB_write_head_y_can_deq_y 
-                                                  CleanQ_RB_write_head_y_can_enq_y
-
- 
-
-
-lemma CleanQ_RB_enq_x_incr_inv:
-  assumes Inv:" CleanQ_RB_Invariants K rb" and
-          sx: "b \<in> rSX rb \<and> the (((ring (rTXY rb) ) (head (rTXY rb)))) = b" and
-          enq:"CleanQ_RB_enq_x_possible rb" 
-  shows "I1_rb_img (CleanQ_RB_incr_head_x b rb) K"
-  using assms unfolding CleanQ_RB_incr_head_x_def rb_incr_head_def I1_rb_img_def
-  oops
-
-lemma CleanQ_RB_enq_x_equal :
-  shows "CleanQ_RB_enq_x b rb =  (CleanQ_RB_incr_head_x b (CleanQ_RB_write_head_x b rb))"
-  unfolding CleanQ_RB_incr_head_x_def CleanQ_RB_write_head_x_def CleanQ_RB_enq_x_def
-  by (metis CleanQ_RB_enq_x_def CleanQ_RB_incr_head_x_def CleanQ_RB_write_head_x_def
-      CleanQ_split_enq_x_equal)
-
-lemma CleanQ_RB_enq_y_equal :
-  shows "CleanQ_RB_enq_y b rb =  (CleanQ_RB_incr_head_y b (CleanQ_RB_write_head_y b rb))"
-  unfolding CleanQ_RB_incr_head_y_def CleanQ_RB_write_head_y_def CleanQ_RB_enq_y_def
-  by (metis CleanQ_RB_enq_y_def CleanQ_RB_incr_head_y_def CleanQ_RB_write_head_y_def
-      CleanQ_split_enq_y_equal)
-
-lemma CleanQ_RB_enq_x_write_I1:
-  assumes Inv:" CleanQ_RB_Invariants K rb" 
-  shows "I1_rb_img (CleanQ_RB_write_head_x b rb) K"
-  using assms
-  by (metis CleanQ_RB_Invariants_def CleanQ_RB_State.ext_inject CleanQ_RB_State.surjective 
-            CleanQ_RB_State.update_convs(3) CleanQ_RB_write_head_x_def I1_rb_img_def 
-            rb_enq_write_same)
-
-lemma CleanQ_RB_enq_x_write_I2:
-  assumes Inv:" CleanQ_RB_Invariants K rb" 
-  shows "I2_rb_img (CleanQ_RB_write_head_x b rb)"
-  using assms unfolding CleanQ_RB_Invariants_simp CleanQ_RB_write_head_x_def
-  by (smt CleanQ_RB_State.ext_inject CleanQ_RB_State.surjective CleanQ_RB_State.update_convs(3) rb_enq_write_same)
-
-lemma CleanQ_RB_enq_x_write_I3:
-  assumes Inv:" CleanQ_RB_Invariants K rb" 
-  shows "I3_rb_img (CleanQ_RB_write_head_x b rb)"
-  using assms unfolding I3_rb_img_def CleanQ_RB_write_head_x_def
-  by (metis CleanQ_RB_Invariants_def CleanQ_RB_State.ext_inject CleanQ_RB_State.surjective 
-            CleanQ_RB_State.update_convs(3) I3_rb_img_def rb_enq_write_same) 
-
-lemma CleanQ_RB_enq_x_write_I4:
-  assumes Inv:" CleanQ_RB_Invariants K rb" 
-  shows "I4_rb_valid(CleanQ_RB_write_head_x b rb)"
-  using assms unfolding I4_rb_valid_def CleanQ_RB_write_head_x_def
-  by (simp add: CleanQ_RB_Invariants_def I4_rb_valid_def rb_write_preserves_valid)
-
-
-lemma CleanQ_RB_enq_y_write_I1:
-  assumes Inv:" CleanQ_RB_Invariants K rb" 
-  shows "I1_rb_img (CleanQ_RB_write_head_y b rb) K"
-  using assms
-  by (metis CleanQ_RB2List_def CleanQ_RB_Invariants_def CleanQ_RB_State.ext_inject 
-            CleanQ_RB_State.surjective CleanQ_RB_State.update_convs(4) CleanQ_RB_write_head_y_def 
-            I1_rb_img_lift rb_enq_write_same)
- 
-
-
-lemma CleanQ_RB_enq_y_write_I2:
-assumes Inv:" CleanQ_RB_Invariants K rb"  
-  shows "I2_rb_img (CleanQ_RB_write_head_y b rb)"
-  using assms unfolding I2_rb_img_def CleanQ_RB_write_head_y_def
-  by (smt CleanQ_RB_Invariants_def CleanQ_RB_State.ext_inject CleanQ_RB_State.surjective 
-          CleanQ_RB_State.update_convs(1)  CleanQ_RB_State.update_convs(4) I2_rb_img_def 
-          rb_enq_write_same)
-  
-
-lemma CleanQ_RB_enq_y_write_I3:
-assumes Inv:" CleanQ_RB_Invariants K rb" 
-  shows "I3_rb_img (CleanQ_RB_write_head_y b rb)"
-  using assms unfolding I3_rb_img_def CleanQ_RB_write_head_y_def
-  by (metis CleanQ_RB_Invariants_def CleanQ_RB_State.ext_inject CleanQ_RB_State.surjective 
-      CleanQ_RB_State.update_convs(4) I3_rb_img_def rb_enq_write_same)
-  
-lemma CleanQ_RB_enq_y_write_I4:
-assumes Inv:" CleanQ_RB_Invariants K rb" 
-  shows "I4_rb_valid(CleanQ_RB_write_head_y b rb)"
-  using assms unfolding I4_rb_valid_def CleanQ_RB_write_head_y_def
-  by (simp add: CleanQ_RB_Invariants_def I4_rb_valid_def rb_write_preserves_valid)
-  
-
-lemma CleanQ_RB_enq_x_write_inv_all:
-assumes Inv:" CleanQ_RB_Invariants K rb"  
-  shows "CleanQ_RB_Invariants K (CleanQ_RB_write_head_x b rb)"
-  using assms unfolding CleanQ_RB_Invariants_def CleanQ_RB_write_head_x_def
-  by (metis CleanQ_RB_write_head_x_def CleanQ_RB_enq_x_write_I1 CleanQ_RB_enq_x_write_I2 
-      CleanQ_RB_enq_x_write_I3 CleanQ_RB_enq_x_write_I4 Inv)
-  
-lemma CleanQ_RB_enq_y_write_inv_all:
-assumes Inv:" CleanQ_RB_Invariants K rb" 
-  shows "CleanQ_RB_Invariants K (CleanQ_RB_write_head_y b rb)"
-  using assms unfolding CleanQ_RB_Invariants_def CleanQ_RB_write_head_y_def
-  by (metis CleanQ_RB_write_head_y_def CleanQ_RB_enq_y_write_I1 CleanQ_RB_enq_y_write_I2 
-      CleanQ_RB_enq_y_write_I3 CleanQ_RB_enq_y_write_I4 Inv)
-
-lemma CleanQ_RB_write_head_inv_all:
-  "CleanQ_RB_Invariants K rb \<longleftrightarrow> CleanQ_RB_Invariants K (CleanQ_RB_write_head_y b rb)"
-  apply(auto simp:CleanQ_RB_enq_y_write_inv_all)
-  unfolding CleanQ_RB_Invariants_def CleanQ_RB_write_head_y_def
-  apply(auto)
-     apply(simp add: I1_rb_img_def) apply (metis rb_enq_write_same)
-    apply(simp add: I2_rb_img_def) apply (metis rb_enq_write_same)
-   apply(simp add: I3_rb_img_def) apply (metis rb_enq_write_same)
-  apply(simp add:I4_rb_valid_def) by (meson rb_write_head_valid)
-  
-
-lemma CleanQ_RB_enq_x_preserves_invariants : 
-  "\<Gamma>\<turnstile> \<lbrace> rb' = \<acute>RingCRB \<and> CleanQ_RB_Invariants K \<acute> RingCRB \<and> b \<in> rSX \<acute> RingCRB \<and>
-         CleanQ_RB_enq_x_possible \<acute>RingCRB \<rbrace> 
-        \<acute>RingCRB :== (CleanQ_RB_write_head_x b \<acute>RingCRB) ;;
-        \<acute>RingCRB :== (CleanQ_RB_incr_head_x b \<acute>RingCRB)
-      \<lbrace> CleanQ_RB_Invariants K \<acute>RingCRB \<rbrace>"
-  apply(vcg)
-  using CleanQ_split_enq_x_equal
-  by (metis CleanQ_RB_enq_x_inv_all) 
-  
-lemma CleanQ_RB_enq_y_preserves_invariants : 
-  "\<Gamma>\<turnstile> \<lbrace> rb' = \<acute>RingCRB \<and> CleanQ_RB_Invariants K \<acute> RingCRB \<and> b \<in> rSY \<acute> RingCRB \<and>
-         CleanQ_RB_enq_y_possible \<acute>RingCRB \<rbrace> 
-        \<acute>RingCRB :== (CleanQ_RB_write_head_y b \<acute>RingCRB) ;;
-        \<acute>RingCRB :== (CleanQ_RB_incr_head_y b \<acute>RingCRB)
-      \<lbrace> CleanQ_RB_Invariants K \<acute>RingCRB \<rbrace>"
-  apply(vcg)
-  using CleanQ_split_enq_y_equal
-  by (metis CleanQ_RB_enq_y_inv_all)   
-
-
-
-
-
-
-
-
 
 lemma CleanQ_RB_head_write_x_not_none:
   "\<not>CleanQ_RB_head_none_x (CleanQ_RB_write_head_x b rb)"
@@ -547,69 +353,270 @@ lemma CleanQ_RB_write_head_read_head_y:
   unfolding CleanQ_RB_read_head_y_def CleanQ_RB_write_head_y_def
   by (simp add: rb_read_head_def rb_write_head_element_read)
 
+
+text \<open>
+  We first show, that the combination of the two operation, yields the original 
+  \verb+enqueue+ operation of the sequential ring buffer model. We add those two to
+  the simp set.
+\<close>
+
+lemma CleanQ_RB_enq_x_split_equal[simp]:
+  "CleanQ_RB_incr_head_x b (CleanQ_RB_write_head_x b rb) = CleanQ_RB_enq_x b rb"
+  unfolding CleanQ_RB_incr_head_x_def CleanQ_RB_write_head_x_def CleanQ_RB_enq_x_def
+  rb_enq_def by simp
+
+lemma CleanQ_RB_enq_y_split_equal[simp]:
+  "CleanQ_RB_incr_head_y b (CleanQ_RB_write_head_y b rb) = CleanQ_RB_enq_y b rb"
+  unfolding CleanQ_RB_incr_head_y_def CleanQ_RB_write_head_y_def CleanQ_RB_enq_y_def
+  rb_enq_def by simp
+
+
+text \<open>
+  Secondly, we can show that if the head of the ring contains some buffer $b$, then 
+  just incrementing the head pointer, results in an equivalent state as when we
+  enqueue this buffer. Note, due to the definitions of reading the head element, 
+  we need to have an additional assumption, that the head is actually not none. 
+
+  We show that writing the head with the same element that currently there, yields the
+  same state. Note, this is trivial, but a proof is required due to the definition of
+  the read operation.
+\<close>
+
+lemma CleanQ_RB_write_head_x_equiv:
+assumes notnone: "\<not>CleanQ_RB_head_none_x rb"  and buf: "b = (CleanQ_RB_read_head_x rb)"
+  shows "CleanQ_RB_write_head_x b rb = rb"
+  using assms 
+  unfolding CleanQ_RB_write_head_x_def CleanQ_RB_head_none_x_def CleanQ_RB_read_head_x_def
+  by (simp add: rb_write_head_same)
+
+lemma CleanQ_RB_write_head_y_equiv:
+assumes notnone: "\<not>CleanQ_RB_head_none_y rb"  and buf: "b = (CleanQ_RB_read_head_y rb)"
+  shows "CleanQ_RB_write_head_y b rb = rb"
+  using assms 
+  unfolding CleanQ_RB_write_head_y_def CleanQ_RB_head_none_y_def CleanQ_RB_read_head_y_def
+  by (simp add: rb_write_head_same)
+
+
+text \<open>
+  Using the state equivalence, we can now show that we can simply increment the head 
+  which yields the same as if we were to do a full \verb+enqueue+ operation.
+\<close>
+
 lemma CleanQ_RB_enq_x_equiv_incr_head:
-  "\<not>CleanQ_RB_head_none_x rb  \<Longrightarrow> b = (CleanQ_RB_read_head_x rb) \<Longrightarrow> (CleanQ_RB_incr_head_x b rb) = CleanQ_RB_enq_x b rb"
-proof -
-  assume buf : "b = (CleanQ_RB_read_head_x rb)"
-  assume notnone: "\<not>CleanQ_RB_head_none_x rb" 
+assumes notnone: "\<not>CleanQ_RB_head_none_x rb"  and buf: "b = (CleanQ_RB_read_head_x rb)"
+  shows "CleanQ_RB_incr_head_x b rb = CleanQ_RB_enq_x b rb"
+  by (metis CleanQ_RB_enq_x_split_equal CleanQ_RB_write_head_x_equiv buf notnone)
 
-  from buf have x1:
-    "rb_read_head ((rTXY rb)) = b"
-    unfolding CleanQ_RB_read_head_x_def by(auto)
-
-  from x1 have x2:
-    "ring (rTXY (rb::'a CleanQ_RB_State)) (head (rTXY rb)) = Some b"
-    using notnone unfolding rb_read_head_def apply(auto) 
-    by (simp add: CleanQ_RB_head_none_x_def rb_head_none_def)
-
-   from x2 have x3: "rb_write_head b (rTXY rb) = (rTXY rb)"
-    unfolding rb_read_head_def 
-    by (metis CleanQ_RB.surjective CleanQ_RB.update_convs(1) fun_upd_triv rb_write_head_def)
-
-  have rbeq:
-    "rb_enq b (rTXY rb) =  rb_incr_head (rTXY rb)"
-    using x3 unfolding rb_enq_def
-    by simp
-
-  show ?thesis
-    using rbeq unfolding CleanQ_RB_enq_x_def CleanQ_RB_incr_head_x_def
-    by(auto)
-qed
+lemma CleanQ_RB_enq_y_equiv_incr_head:
+assumes notnone: "\<not>CleanQ_RB_head_none_y rb"  and buf: "b = (CleanQ_RB_read_head_y rb)"
+  shows "CleanQ_RB_incr_head_y b rb = CleanQ_RB_enq_y b rb"
+  by (metis CleanQ_RB_enq_y_split_equal CleanQ_RB_write_head_y_equiv buf notnone)
 
 
+text \<open>
+  Just writing the head element in the ring, does not change the state when its lifted
+  to the list model. 
+\<close>
+
+lemma CleanQ_RB_write_head_x_list[simp]:
+  "CleanQ_RB_list (rTXY (CleanQ_RB_write_head_x b rb)) = CleanQ_RB_list (rTXY rb)"
+  by (metis CleanQ_RB_State.ext_inject CleanQ_RB_State.surjective rb_enq_write_same
+            CleanQ_RB_State.update_convs(3) CleanQ_RB_write_head_x_def)
+    
+lemma CleanQ_RB_write_head_y_list[simp]:
+ "CleanQ_RB_list (rTYX (CleanQ_RB_write_head_y b rb)) = CleanQ_RB_list (rTYX rb)"
+  by (metis CleanQ_RB_State.ext_inject CleanQ_RB_State.surjective rb_enq_write_same
+            CleanQ_RB_State.update_convs(4) CleanQ_RB_write_head_y_def)
 
 
-abbreviation "CleanQ_Enq_X_P K rb b \<equiv> CleanQ_RB_Invariants K rb \<and> CleanQ_RB_enq_x_possible rb \<and> b \<in> rSX rb"
-abbreviation "CleanQ_Enq_X_Q K rb b \<equiv> CleanQ_RB_Invariants K rb \<and> CleanQ_RB_enq_x_possible rb \<and> b \<in> rSX rb \<and>  b = CleanQ_RB_read_head_x rb \<and> \<not>CleanQ_RB_head_none_x rb "
-abbreviation "CleanQ_Enq_X_R K rb b \<equiv> CleanQ_RB_Invariants K rb"
+text \<open>
+  The entire lifted state to the list model is not changed at all.  
+\<close>
 
-abbreviation "CleanQ_Enq_Y_P K rb b \<equiv> CleanQ_RB_Invariants K rb \<and> CleanQ_RB_enq_y_possible rb \<and> b \<in> rSY rb"
-abbreviation "CleanQ_Enq_Y_Q K rb b \<equiv> CleanQ_RB_Invariants K rb \<and> CleanQ_RB_enq_y_possible rb \<and> b \<in> rSY rb \<and>  b = CleanQ_RB_read_head_y rb \<and> \<not>CleanQ_RB_head_none_y rb "
-abbreviation "CleanQ_Enq_Y_R K rb b \<equiv> CleanQ_RB_Invariants K rb"
+lemma CleanQ_RB_write_head_x_lift_full:
+  "CleanQ_RB2List (CleanQ_RB_write_head_x b rb) = CleanQ_RB2List rb"
+  unfolding CleanQ_RB2List_def by (simp, auto simp: CleanQ_RB_write_head_x_def)
 
-
-
-
-abbreviation "CleanQ_Deq_X_P K rb b \<equiv> CleanQ_RB_Invariants K rb \<and> CleanQ_RB_deq_x_possible rb"
-abbreviation "CleanQ_Deq_X_Q K rb b \<equiv> CleanQ_RB_Invariants K rb \<and> CleanQ_RB_deq_x_possible rb \<and> b = CleanQ_RB_read_tail_x rb"
-abbreviation "CleanQ_Deq_X_R K rb b \<equiv> CleanQ_RB_Invariants K rb"
+lemma CleanQ_RB_write_head_y_lift_full:
+  "CleanQ_RB2List (CleanQ_RB_write_head_y b rb) = CleanQ_RB2List rb"
+  unfolding CleanQ_RB2List_def by (simp, auto simp: CleanQ_RB_write_head_y_def)
 
 
+text \<open>
+  Writing the head preserves all \verb+can_enq+ and \verb+can_deq+ predicates. 
+\<close>
 
-lemma  CleanQ_RB_write_head_x_hoare:
-  "\<Gamma>\<turnstile> \<lbrace> CleanQ_Enq_X_P K \<acute>RingCRB b \<rbrace> 
-        \<acute>RingCRB :== (CleanQ_RB_write_head_x b \<acute>RingCRB)
-      \<lbrace> CleanQ_Enq_X_Q K \<acute> RingCRB b  \<rbrace>"
-  apply(vcg, auto simp: CleanQ_RB_enq_x_write_inv_all CleanQ_RB_enq_x_write_can_enq 
-                        CleanQ_RB_write_head_read_head_x CleanQ_RB_head_write_x_not_none)
-  by(simp add: CleanQ_RB_write_head_x_def)
+lemma CleanQ_RB_write_head_y_can_enq_x:
+  "CleanQ_RB_enq_x_possible rb = CleanQ_RB_enq_x_possible (CleanQ_RB_write_head_y b rb)"
+  by (simp add: CleanQ_RB_write_head_y_def CleanQ_RB_enq_x_possible_def) 
+
+lemma CleanQ_RB_write_head_y_can_deq_x:
+ "CleanQ_RB_deq_x_possible rb = CleanQ_RB_deq_x_possible (CleanQ_RB_write_head_y b rb)"
+  by(simp add: CleanQ_RB_deq_x_possible_def CleanQ_RB_write_head_y_def rb_write_can_deq)
+
+lemma CleanQ_RB_write_head_y_can_deq_y:
+  "CleanQ_RB_deq_y_possible rb = CleanQ_RB_deq_y_possible (CleanQ_RB_write_head_y b rb)"
+  by (simp add: CleanQ_RB_deq_y_possible_def CleanQ_RB_write_head_y_def)
+
+lemma CleanQ_RB_write_head_y_can_enq_y:
+ "CleanQ_RB_enq_y_possible rb = CleanQ_RB_enq_y_possible (CleanQ_RB_write_head_y b rb)"
+  by(simp add: CleanQ_RB_enq_y_possible_def CleanQ_RB_write_head_y_def rb_write_can_enq)
 
 
-lemma  CleanQ_RB_incr_head_x_hoare:
-  "\<Gamma>\<turnstile> \<lbrace>  CleanQ_Enq_X_Q K \<acute>RingCRB b \<rbrace> 
-        \<acute>RingCRB :== (CleanQ_RB_incr_head_x b \<acute>RingCRB)
-      \<lbrace> CleanQ_Enq_X_R K \<acute> RingCRB b  \<rbrace>"
-  by(vcg, simp add: CleanQ_RB_enq_x_equiv_incr_head CleanQ_RB_enq_x_inv_all)
+lemma CleanQ_RB_write_head_x_can_enq_x:
+  "CleanQ_RB_enq_x_possible rb = CleanQ_RB_enq_x_possible (CleanQ_RB_write_head_x b rb)"
+  by(simp add: CleanQ_RB_write_head_x_def CleanQ_RB_enq_x_possible_def rb_write_can_enq)
+
+lemma CleanQ_RB_write_head_x_can_deq_x:
+ "CleanQ_RB_deq_x_possible rb = CleanQ_RB_deq_x_possible (CleanQ_RB_write_head_x b rb)"
+  by(simp add: CleanQ_RB_deq_x_possible_def CleanQ_RB_write_head_x_def rb_write_can_deq)
+
+lemma CleanQ_RB_write_head_x_can_deq_y:
+  "CleanQ_RB_deq_y_possible rb = CleanQ_RB_deq_y_possible (CleanQ_RB_write_head_x b rb)"
+  by(simp add: CleanQ_RB_deq_y_possible_def CleanQ_RB_write_head_x_def rb_write_can_deq)
+
+lemma CleanQ_RB_write_head_x_can_enq_y:
+ "CleanQ_RB_enq_y_possible rb = CleanQ_RB_enq_y_possible (CleanQ_RB_write_head_x b rb)"
+  by(simp add: CleanQ_RB_enq_y_possible_def CleanQ_RB_write_head_x_def rb_write_can_enq)
+
+
+
+lemmas CleanQ_RB_write_head_y_can_enq_deq_simps = CleanQ_RB_write_head_y_can_enq_x 
+                                                  CleanQ_RB_write_head_y_can_deq_x 
+                                                  CleanQ_RB_write_head_y_can_deq_y 
+                                                  CleanQ_RB_write_head_y_can_enq_y
+
+lemmas CleanQ_RB_write_head_x_can_enq_deq_simps = CleanQ_RB_write_head_x_can_enq_x 
+                                                  CleanQ_RB_write_head_x_can_deq_x 
+                                                  CleanQ_RB_write_head_x_can_deq_y 
+                                                  CleanQ_RB_write_head_x_can_enq_y
+ 
+
+text \<open>
+  Next we show that the write operation preserves the invariant. We show this individually, 
+  plus also we show both ways, as a simple write to the ring, does not change anything
+  in the observable state and thus also preserves the invariant.
+\<close>
+
+lemma CleanQ_RB_write_head_x_I1:
+ "I1_rb_img rb K \<longleftrightarrow> I1_rb_img (CleanQ_RB_write_head_x b rb) K"
+  by (simp add: CleanQ_RB_write_head_x_lift_full I1_rb_img_lift)
+
+lemma CleanQ_RB_write_head_x_I2:
+ "I2_rb_img rb \<longleftrightarrow> I2_rb_img (CleanQ_RB_write_head_x b rb)"
+  by (simp add: CleanQ_RB_write_head_x_lift_full I2_rb_img_lift)
+
+lemma CleanQ_RB_write_head_x_I3:
+  "I3_rb_img rb \<longleftrightarrow> I3_rb_img (CleanQ_RB_write_head_x b rb)"
+  by (simp add:  CleanQ_RB_write_head_x_lift_full I3_rb_img_lift)
+
+lemma CleanQ_RB_write_head_x_I4:
+  "I4_rb_valid rb \<longleftrightarrow> I4_rb_valid (CleanQ_RB_write_head_x b rb)"
+  unfolding I4_rb_valid_def CleanQ_RB_write_head_x_def
+  by(simp, meson rb_write_head_valid)
+
+lemma CleanQ_RB_write_head_x_Invariant[simp]:
+  "CleanQ_RB_Invariants K rb \<longleftrightarrow> CleanQ_RB_Invariants K (CleanQ_RB_write_head_x b rb)"
+  by (meson CleanQ_RB_Invariants_def CleanQ_RB_write_head_x_I1 CleanQ_RB_write_head_x_I2
+            CleanQ_RB_write_head_x_I3 CleanQ_RB_write_head_x_I4)
+
+
+lemma CleanQ_RB_write_head_y_I1:
+ "I1_rb_img rb K \<longleftrightarrow> I1_rb_img (CleanQ_RB_write_head_y b rb) K"
+  by (simp add: CleanQ_RB_write_head_y_lift_full I1_rb_img_lift)
+
+lemma CleanQ_RB_write_head_y_I2:
+ "I2_rb_img rb \<longleftrightarrow> I2_rb_img (CleanQ_RB_write_head_y b rb)"
+  by (simp add: CleanQ_RB_write_head_y_lift_full I2_rb_img_lift)
+
+lemma CleanQ_RB_write_head_y_I3:
+  "I3_rb_img rb \<longleftrightarrow> I3_rb_img (CleanQ_RB_write_head_y b rb)"
+  by (simp add:  CleanQ_RB_write_head_y_lift_full I3_rb_img_lift)
+
+lemma CleanQ_RB_write_head_y_I4:
+  "I4_rb_valid rb \<longleftrightarrow> I4_rb_valid (CleanQ_RB_write_head_y b rb)"
+  unfolding I4_rb_valid_def CleanQ_RB_write_head_y_def
+  by(simp, meson rb_write_head_valid)
+
+lemma CleanQ_RB_write_head_y_Invariant[simp]:
+  "CleanQ_RB_Invariants K rb \<longleftrightarrow> CleanQ_RB_Invariants K (CleanQ_RB_write_head_y b rb)"
+  by (meson CleanQ_RB_Invariants_def CleanQ_RB_write_head_y_I1 CleanQ_RB_write_head_y_I2
+            CleanQ_RB_write_head_y_I3 CleanQ_RB_write_head_y_I4)
+
+
+(* ------------------------------------------------------------------------------------ *)
+subsubsection \<open>Pre-Post Conditions for the Enqueue Operation\<close>
+(* ------------------------------------------------------------------------------------ *)
+
+
+text \<open>
+  We now define the hoare triples for the enqueue operation. Those are needed to later
+  for the interference proof. There are a total of three predicates for the enqueue
+  operation in small step semantics, while the predicates P and R define the big 
+  step semantics.
+
+  \verb+{P} write_head {Q} incr_head {R}+ 
+
+  We now provide abbreviations for each of the predicate P, Q, and R for the \verb+enqueue+
+  operation as seen from Y and X.   
+\<close>
+
+paragraph \<open>Enqueue P\<close>
+
+text \<open>
+  The P predicate is the pre-condition for the \verb+enqueue+ operation. For the operation
+  to succeed, the state must satisfy the Invariant plus an enqueue must be possible, i.e.
+  there is space in the descriptor ring to hold the buffer. Lastly, the buffer to be 
+  enqueued must be owned by the agent i.e. a member of the set SX or SY respectively.
+  We provide two abbreviations for this, one for each side:\<close>
+
+abbreviation "CleanQ_RB_enq_x_P K rb b \<equiv> CleanQ_RB_Invariants K rb \<and> 
+                                          CleanQ_RB_enq_x_possible rb \<and> b \<in> rSX rb"
+
+abbreviation "CleanQ_RB_enq_y_P K rb b \<equiv> CleanQ_RB_Invariants K rb \<and> 
+                                          CleanQ_RB_enq_y_possible rb \<and> b \<in> rSY rb"
+
+paragraph \<open>Enqueue Q\<close>
+
+text \<open>
+  The Q predicate is the post-condition for the write part of the  \verb+enqueue+ operation, 
+  and the pre-condition of the increment part of the \verb+enqueue+ operation. The write
+  operation does not transfer ownership of the buffer yet, thus the buffer remains in
+  SX or SY respectively and the enqueue still remains possible. However, we now know, 
+  that the buffer is written to the head location of the ring, and that this location
+  is not \verb+None+.
+\<close>
+
+abbreviation "CleanQ_RB_enq_x_Q K rb b \<equiv> CleanQ_RB_Invariants K rb \<and> 
+                                          CleanQ_RB_enq_x_possible rb \<and> b \<in> rSX rb \<and> 
+                                          b = CleanQ_RB_read_head_x rb \<and> 
+                                          \<not>CleanQ_RB_head_none_x rb "
+
+abbreviation "CleanQ_RB_enq_y_Q K rb b \<equiv> CleanQ_RB_Invariants K rb \<and> 
+                                          CleanQ_RB_enq_y_possible rb \<and> b \<in> rSY rb \<and>
+                                           b = CleanQ_RB_read_head_y rb \<and> 
+                                           \<not>CleanQ_RB_head_none_y rb "
+
+paragraph \<open>Enqueue R\<close>
+
+
+text \<open>
+  The R predicate is the post condition for both, the increment head part as well as the
+  full \verb+enqueue+ operation. We now that the buffer is now no longer in the owning 
+  sets SX and SY. Note, we cannot make a state about whether it is in the ring, because
+  the other side may have already taken it out. Also, we cannot make any statements
+  about whether we can enqueue again.
+\<close>
+
+abbreviation "CleanQ_RB_enq_y_R K rb b \<equiv> CleanQ_RB_Invariants K rb \<and> b \<notin> rSX rb"
+abbreviation "CleanQ_RB_enq_x_R K rb b \<equiv> CleanQ_RB_Invariants K rb \<and> b \<notin> rSY rb"
+
+
+
+
+
+
+
   
 
 
@@ -670,8 +677,18 @@ lemma CleanQ_RB_deq_y_preserves_invariants :
   using CleanQ_split_deq_y_equal
   by (metis CleanQ_RB_deq_y_all_inv) 
 
+
+
+
+abbreviation "CleanQ_Deq_X_P K rb b \<equiv> CleanQ_RB_Invariants K rb \<and> CleanQ_RB_deq_x_possible rb"
+abbreviation "CleanQ_Deq_X_Q K rb b \<equiv> CleanQ_RB_Invariants K rb \<and> CleanQ_RB_deq_x_possible rb \<and> b = CleanQ_RB_read_tail_x rb"
+abbreviation "CleanQ_Deq_X_R K rb b \<equiv> CleanQ_RB_Invariants K rb"
+
+
+
+
 (* ------------------------------------------------------------------------------------ *)
-subsubsection \<open>Invariants are TRUE invariants\<close>
+subsection \<open>Invariants are TRUE invariants\<close>
 (* ------------------------------------------------------------------------------------ *)
 text \<open>
   To show that the Invariants we defined are true invariants it has to hold at each
@@ -679,57 +696,125 @@ text \<open>
   we will show the invariant for each of the two steps of \verb+enqueue+ and \verb+dequeue+. 
 \<close>
 
-lemma CleanQ_CRB_write_enq_x_preserves_invariants : 
-  "\<Gamma>\<turnstile> \<lbrace> rb' = \<acute>RingCRB \<and> CleanQ_RB_Invariants K \<acute> RingCRB \<and> b \<in> rSX \<acute> RingCRB \<and>
-         CleanQ_RB_enq_x_possible \<acute>RingCRB \<rbrace> 
+
+
+(* ------------------------------------------------------------------------------------ *)
+subsubsection \<open>Hoare Triples for the Enqueue Operation\<close>
+(* ------------------------------------------------------------------------------------ *)
+
+
+text \<open>
+  We now show that the \verb+enqueue+ operation satisfies the pre and post conditions
+  for the predicates P, Q and R. 
+\<close>
+
+
+paragraph \<open>Writing the Head Element\<close>
+
+text \<open>
+  We show the Hoare triple with \verb+{P) write_head {Q}+.
+\<close>
+
+lemma  CleanQ_RB_write_head_x_hoare:
+  "\<Gamma>\<turnstile> \<lbrace> CleanQ_RB_enq_x_P K \<acute>RingCRB b \<rbrace> 
         \<acute>RingCRB :== (CleanQ_RB_write_head_x b \<acute>RingCRB)
-      \<lbrace> CleanQ_RB_Invariants K \<acute> RingCRB \<and> b \<in> rSX \<acute> RingCRB \<and> 
-        CleanQ_RB_enq_x_possible \<acute>RingCRB \<and> b = the (((ring (rTXY \<acute>RingCRB) ) (head (rTXY \<acute>RingCRB))))\<rbrace>"
-  apply(vcg)
-  unfolding CleanQ_RB_enq_x_possible_def rb_can_enq_def 
-    CleanQ_RB_write_head_x_def rb_write_head_def
-proof -
-  fix RingCRB :: "nat CleanQ_RB_State"
-  assume a1: "\<not> rb_full (rTXY RingCRB)"
-  assume a2: "b \<in> rSX RingCRB"
-  assume a3: "CleanQ_RB_Invariants K RingCRB"
-  have "rb_can_enq (rTXY RingCRB)"
-    using a1 rb_can_enq_def by blast
-  then have "CleanQ_RB_enq_x_possible RingCRB"
-    by (simp add: CleanQ_RB_enq_x_possible_def)
-  then show "CleanQ_RB_Invariants K (RingCRB \<lparr>rTXY := rTXY RingCRB \<lparr>ring := ring (rTXY RingCRB)(head (rTXY RingCRB) \<mapsto> b)\<rparr>\<rparr>) \<and> b \<in> rSX (RingCRB \<lparr>rTXY := rTXY RingCRB \<lparr>ring := ring (rTXY RingCRB) (head (rTXY RingCRB) \<mapsto> b)\<rparr>\<rparr>) \<and> \<not> rb_full (rTXY (RingCRB \<lparr>rTXY := rTXY RingCRB \<lparr>ring := ring (rTXY RingCRB) (head (rTXY RingCRB) \<mapsto> b)\<rparr>\<rparr>)) \<and> b = the (ring (rTXY (RingCRB \<lparr>rTXY := rTXY RingCRB \<lparr>ring := ring (rTXY RingCRB)(head (rTXY RingCRB) \<mapsto> b)\<rparr>\<rparr>)) (head (rTXY (RingCRB \<lparr>rTXY := rTXY RingCRB \<lparr>ring := ring (rTXY RingCRB) (head (rTXY RingCRB) \<mapsto> b)\<rparr>\<rparr>))))"
-    using a3 a2 by (metis (no_types) CleanQ_RB_State.select_convs(1) CleanQ_RB_State.select_convs(3) CleanQ_RB_State.surjective CleanQ_RB_State.update_convs(1) CleanQ_RB_State.update_convs(3) CleanQ_RB_write_head_x_def CleanQ_RB_enq_x_possible_def CleanQ_RB_enq_x_write_can_enq CleanQ_RB_enq_x_write_inv_all option.sel rb_can_enq_def rb_write_head_def rb_write_head_element)
-qed 
+      \<lbrace> CleanQ_RB_enq_x_Q K \<acute> RingCRB b  \<rbrace>"                                                 
+  apply(vcg, auto simp: CleanQ_RB_write_head_x_Invariant[symmetric] 
+                        CleanQ_RB_write_head_x_can_enq_x[symmetric]
+                        CleanQ_RB_write_head_read_head_x CleanQ_RB_head_write_x_not_none)
+  by(simp add: CleanQ_RB_write_head_x_def)
 
-lemma CleanQ_CRB_write_enq_y_preserves_invariants : 
-  "\<Gamma>\<turnstile> \<lbrace> rb' = \<acute>RingCRB \<and> CleanQ_RB_Invariants K \<acute> RingCRB \<and> b \<in> rSY \<acute> RingCRB \<and>
-         CleanQ_RB_enq_y_possible \<acute>RingCRB \<rbrace> 
+
+lemma  CleanQ_RB_write_head_y_hoare:
+  "\<Gamma>\<turnstile> \<lbrace> CleanQ_RB_enq_y_P K \<acute>RingCRB b \<rbrace> 
         \<acute>RingCRB :== (CleanQ_RB_write_head_y b \<acute>RingCRB)
-      \<lbrace> CleanQ_RB_Invariants K \<acute> RingCRB \<and> b \<in> rSY \<acute> RingCRB \<and> 
-        CleanQ_RB_enq_y_possible \<acute>RingCRB \<and> b = the (((ring (rTYX \<acute>RingCRB) ) (head (rTYX \<acute>RingCRB))))\<rbrace>"
-  apply(vcg)
-  unfolding CleanQ_RB_enq_y_possible_def rb_can_enq_def 
-    CleanQ_RB_write_head_y_def rb_write_head_def
-  apply auto
-  apply (smt CleanQ_RB.ext_inject CleanQ_RB.surjective CleanQ_RB.update_convs(1) 
-         CleanQ_RB_Invariants_def CleanQ_RB_State.select_convs(1) CleanQ_RB_State.select_convs(2) 
-         CleanQ_RB_State.select_convs(3) CleanQ_RB_State.select_convs(4) CleanQ_RB_State.surjective 
-         CleanQ_RB_State.update_convs(4) CleanQ_RB_list_def I1_rb_img_def I2_rb_img_def I3_rb_img_def 
-         I4_rb_valid_def fun_upd_other map_fun_upd map_map rb_valid_def rb_valid_entries_def 
-         rb_valid_ptr_def rb_write_head_element_notin_valid)
-  by (simp add: rb_full_def)
+      \<lbrace> CleanQ_RB_enq_y_Q K \<acute> RingCRB b  \<rbrace>"                                                 
+  apply(vcg, auto simp: CleanQ_RB_write_head_y_Invariant[symmetric] 
+                        CleanQ_RB_write_head_y_can_enq_y[symmetric]
+                        CleanQ_RB_write_head_read_head_y CleanQ_RB_head_write_y_not_none)
+  by(simp add: CleanQ_RB_write_head_y_def)
 
-(*
-lemma CleanQ_CRB_incr_enq_x_preserves_invariants : 
-  "\<Gamma>\<turnstile> \<lbrace> CleanQ_RB_Invariants K rb \<and> b \<in> rSX rb \<and> 
-        CleanQ_RB_enq_x_possible rb \<and>\<acute>RingCRB = (CleanQ_RB_write_head_y b rb)\<rbrace>
+
+paragraph \<open>Incrementing the Head Pointer\<close>
+
+text \<open>
+  We show the Hoare triple with \verb+{Q) incr_head {R}+.
+\<close>
+
+lemma  CleanQ_RB_incr_head_x_hoare:
+  "\<Gamma>\<turnstile> \<lbrace>  CleanQ_RB_enq_x_Q K \<acute>RingCRB b \<rbrace> 
         \<acute>RingCRB :== (CleanQ_RB_incr_head_x b \<acute>RingCRB)
-      \<lbrace> CleanQ_RB_Invariants K \<acute> RingCRB\<rbrace>"
-  apply(vcg) 
-  using CleanQ_RB_enq_x_equal CleanQ_RB_enq_x_inv_all
-  apply auto
-  *)
+      \<lbrace> CleanQ_RB_enq_x_R K \<acute> RingCRB b  \<rbrace>"
+  apply(vcg, simp add: CleanQ_RB_enq_x_equiv_incr_head CleanQ_RB_enq_x_inv_all)
+  by (simp add: CleanQ_RB_enq_x_result)
+
+lemma  CleanQ_RB_incr_head_y_hoare:
+  "\<Gamma>\<turnstile> \<lbrace>  CleanQ_RB_enq_y_Q K \<acute>RingCRB b \<rbrace> 
+        \<acute>RingCRB :== (CleanQ_RB_incr_head_y b \<acute>RingCRB)
+      \<lbrace> CleanQ_RB_enq_y_R K \<acute> RingCRB b  \<rbrace>"
+  apply(vcg, simp add: CleanQ_RB_enq_y_equiv_incr_head CleanQ_RB_enq_y_inv_all)
+  by (simp add: CleanQ_RB_enq_y_result)
+
+
+paragraph \<open>Full Enqueue Operation\<close>
+
+text \<open>
+  We show the Hoare triple with \verb+{P) enq {R}+.
+\<close>
+
+lemma CleanQ_RB_enq_x_hoare : 
+  "\<Gamma>\<turnstile> \<lbrace> CleanQ_RB_enq_x_P K \<acute>RingCRB b \<rbrace> 
+        \<acute>RingCRB :== (CleanQ_RB_write_head_x b \<acute>RingCRB) ;;
+        \<acute>RingCRB :== (CleanQ_RB_incr_head_x b \<acute>RingCRB)
+      \<lbrace> CleanQ_RB_enq_x_R K \<acute>RingCRB b \<rbrace>"
+  apply(vcg) using CleanQ_RB_enq_x_inv_all CleanQ_RB_enq_x_result by fastforce
  
+
+lemma CleanQ_RB_enq_y_hoare : 
+  "\<Gamma>\<turnstile> \<lbrace> CleanQ_RB_enq_y_P K \<acute>RingCRB b \<rbrace> 
+        \<acute>RingCRB :== (CleanQ_RB_write_head_y b \<acute>RingCRB) ;;
+        \<acute>RingCRB :== (CleanQ_RB_incr_head_y b \<acute>RingCRB)
+      \<lbrace> CleanQ_RB_enq_y_R K \<acute>RingCRB b \<rbrace>"
+  apply(vcg) using CleanQ_RB_enq_y_inv_all CleanQ_RB_enq_y_result by fastforce
+
+
+
+(* ------------------------------------------------------------------------------------ *)
+subsubsection \<open>Hoare Triples for the Dequeue Operation\<close>
+(* ------------------------------------------------------------------------------------ *)
+
+
+text \<open>
+  We now show that the \verb+dequeue+ operation satisfies the pre and post conditions
+  for the predicates P, Q and R. 
+\<close>
+
+
+paragraph \<open>Reading the Tail Element\<close>
+
+text \<open>
+  We show the Hoare triple with \verb+{P) read_tail {Q}+.
+\<close>
+
+
+
+
+paragraph \<open>Incrementing the Tail Pointer\<close>
+
+text \<open>
+  We show the Hoare triple with \verb+{Q) incr_tail {R}+.
+\<close>
+
+
+
+paragraph \<open>Full Dequeue Operation\<close>
+
+text \<open>
+  We show the Hoare triple with \verb+{P) deq {R}+.
+\<close>
+
+
+
   
 
 
@@ -763,6 +848,7 @@ lemma CleanQ_RB_incr_deq_y_preserves_invariants :
       \<lbrace> CleanQ_RB_Invariants K \<acute>RingCRB \<rbrace>"
     apply vcg
   by (metis CleanQ_RB_deq_y_all_inv CleanQ_split_deq_y_equal)
+
 
 (* ------------------------------------------------------------------------------------ *)
 subsubsection \<open>Weak frame condition preserver invariants\<close>
@@ -1015,54 +1101,65 @@ text \<open>
 paragraph \<open>Y writes the descriptor ring\<close>
 
 lemma CleanQ_CRB_Enqueue_X_P_write_head:
-"\<Gamma>\<turnstile> \<lbrace> CleanQ_Enq_X_P K \<acute>RingCRB bx  \<rbrace> 
+"\<Gamma>\<turnstile> \<lbrace> CleanQ_RB_enq_x_P K \<acute>RingCRB bx  \<rbrace> 
    \<acute>RingCRB :== CleanQ_RB_write_head_y b \<acute>RingCRB 
-  \<lbrace>  CleanQ_Enq_X_P K \<acute>RingCRB bx  \<rbrace>"
-  apply(vcg, simp add:CleanQ_RB_enq_y_write_inv_all CleanQ_RB_write_head_y_can_enq_x[symmetric])  
+  \<lbrace>  CleanQ_RB_enq_x_P K \<acute>RingCRB bx  \<rbrace>"
+  apply(vcg, simp add: CleanQ_RB_write_head_y_can_enq_x[symmetric] CleanQ_RB_write_head_y_Invariant[symmetric])  
   by (simp add: CleanQ_RB_write_head_y_def)
 
 lemma CleanQ_CRB_Enqueue_X_Q_write_head:
-"\<Gamma>\<turnstile> \<lbrace> CleanQ_Enq_X_Q K \<acute>RingCRB bx  \<rbrace> 
+"\<Gamma>\<turnstile> \<lbrace> CleanQ_RB_enq_x_Q K \<acute>RingCRB bx  \<rbrace> 
    \<acute>RingCRB :== CleanQ_RB_write_head_y b \<acute>RingCRB 
-  \<lbrace>  CleanQ_Enq_X_Q K \<acute>RingCRB bx \<rbrace>"
-  apply(vcg, simp add:CleanQ_RB_enq_y_write_inv_all CleanQ_RB_write_head_y_can_enq_x[symmetric])
-  by(simp add: CleanQ_RB_write_head_y_def CleanQ_RB_read_head_x_def )
+  \<lbrace>  CleanQ_RB_enq_x_Q K \<acute>RingCRB bx \<rbrace>"
+  apply(vcg, auto simp add: CleanQ_RB_write_head_y_can_enq_x[symmetric]
+                            CleanQ_RB_write_head_y_Invariant[symmetric])
+ 
+  apply (simp add: CleanQ_RB_write_head_y_def)
+  apply (simp add: CleanQ_RB_read_head_x_def CleanQ_RB_write_head_y_def)
+  by (simp add: CleanQ_RB_head_none_x_def CleanQ_RB_write_head_y_def)
+
 
 lemma CleanQ_CRB_Enqueue_X_R_write_head:
-"\<Gamma>\<turnstile> \<lbrace> CleanQ_Enq_X_R K \<acute>RingCRB bx  \<rbrace> 
+"\<Gamma>\<turnstile> \<lbrace> CleanQ_RB_enq_x_R K \<acute>RingCRB bx  \<rbrace> 
    \<acute>RingCRB :== CleanQ_RB_write_head_y b \<acute>RingCRB 
-  \<lbrace>  CleanQ_Enq_X_R K \<acute>RingCRB bx \<rbrace>"
-   by(vcg, simp add:CleanQ_RB_enq_y_write_inv_all)  
+  \<lbrace>  CleanQ_RB_enq_x_R K \<acute>RingCRB bx \<rbrace>"
+  apply(vcg, auto simp:CleanQ_RB_write_head_y_Invariant[symmetric])  
+  by (simp add: CleanQ_RB_write_head_y_def)
+
+
+  
 
 paragraph \<open>Y increments the head\<close>
 
 lemma CleanQ_CRB_Enqueue_X_P_incr_head:
-"\<Gamma>\<turnstile> \<lbrace>  rb = CleanQ_RB_write_head_y b \<acute>RingCRB \<and> b \<in> rSY \<acute>RingCRB \<and> CleanQ_RB_enq_y_possible \<acute>RingCRB \<and> CleanQ_Enq_X_P K rb bx  \<rbrace> 
+"\<Gamma>\<turnstile> \<lbrace>  rb = CleanQ_RB_write_head_y b \<acute>RingCRB \<and> b \<in> rSY \<acute>RingCRB \<and> CleanQ_RB_enq_y_possible \<acute>RingCRB \<and> CleanQ_RB_enq_x_P K rb bx  \<rbrace> 
    \<acute>RingCRB :== CleanQ_RB_incr_head_y b rb 
-  \<lbrace>  CleanQ_Enq_X_P K \<acute>RingCRB bx  \<rbrace>"
+  \<lbrace>  CleanQ_RB_enq_x_P K \<acute>RingCRB bx  \<rbrace>"
   apply(vcg, auto)
-  apply (meson CleanQ_RB_enq_y_inv_all CleanQ_RB_write_head_inv_all)
-  apply (meson CleanQ_RB_enq_y_enq_x_possible CleanQ_RB_write_head_inv_all CleanQ_RB_write_head_y_can_enq_x)
+    apply (meson CleanQ_RB_enq_y_inv_all CleanQ_RB_write_head_y_Invariant)
+  apply (meson CleanQ_RB_enq_y_enq_x_possible CleanQ_RB_write_head_y_Invariant CleanQ_RB_write_head_y_can_enq_x)
   by (simp add: CleanQ_RB_enq_y_def CleanQ_RB_write_head_y_def)
 
 
 lemma CleanQ_CRB_Enqueue_X_Q_incr_head:
-"\<Gamma>\<turnstile> \<lbrace>  rb = CleanQ_RB_write_head_y b \<acute>RingCRB \<and> b \<in> rSY \<acute>RingCRB \<and> CleanQ_RB_enq_y_possible \<acute>RingCRB \<and> CleanQ_Enq_X_Q K rb bx   \<rbrace> 
+"\<Gamma>\<turnstile> \<lbrace>  rb = CleanQ_RB_write_head_y b \<acute>RingCRB \<and> b \<in> rSY \<acute>RingCRB \<and> CleanQ_RB_enq_y_possible \<acute>RingCRB \<and> CleanQ_RB_enq_x_Q K rb bx   \<rbrace> 
    \<acute>RingCRB :== CleanQ_RB_incr_head_y b rb 
-  \<lbrace>  CleanQ_Enq_X_Q K \<acute>RingCRB bx \<rbrace>"
+  \<lbrace>  CleanQ_RB_enq_x_Q K \<acute>RingCRB bx \<rbrace>"
   apply(vcg, auto)
-  apply (meson CleanQ_RB_enq_y_inv_all CleanQ_RB_write_head_inv_all)
-  apply (meson CleanQ_RB_enq_y_enq_x_possible CleanQ_RB_write_head_inv_all CleanQ_RB_write_head_y_can_enq_x)
-  apply (simp add: CleanQ_RB_enq_y_def CleanQ_RB_write_head_y_def)
-  by (simp add: CleanQ_RB_enq_y_def CleanQ_RB_read_head_x_def CleanQ_RB_write_head_y_def)
+  apply (meson CleanQ_RB_enq_y_inv_all CleanQ_RB_write_head_y_Invariant)
+  apply (meson CleanQ_RB_enq_y_enq_x_possible CleanQ_RB_write_head_y_Invariant CleanQ_RB_write_head_y_can_enq_x)
+    apply (simp add: CleanQ_RB_enq_y_def CleanQ_RB_write_head_y_def)
+   apply (simp add: CleanQ_RB_enq_y_def CleanQ_RB_read_head_x_def CleanQ_RB_write_head_y_def)
+  by (simp add: CleanQ_RB_enq_y_def CleanQ_RB_head_none_x_def CleanQ_RB_write_head_y_def)
+  
   
 lemma CleanQ_CRB_Enqueue_X_R_incr_head:
-"\<Gamma>\<turnstile> \<lbrace> rb = CleanQ_RB_write_head_y b \<acute>RingCRB \<and> b \<in> rSY \<acute>RingCRB \<and> CleanQ_RB_enq_y_possible \<acute>RingCRB \<and> CleanQ_Enq_X_R K rb bx  \<rbrace> 
+"\<Gamma>\<turnstile> \<lbrace> rb = CleanQ_RB_write_head_y b \<acute>RingCRB \<and> b \<in> rSY \<acute>RingCRB \<and> CleanQ_RB_enq_y_possible \<acute>RingCRB \<and> CleanQ_RB_enq_x_R K rb bx  \<rbrace> 
    \<acute>RingCRB :== CleanQ_RB_incr_head_y b rb 
-  \<lbrace>  CleanQ_Enq_X_R K \<acute>RingCRB bx \<rbrace>"
+  \<lbrace>  CleanQ_RB_enq_x_R K \<acute>RingCRB bx \<rbrace>"
   apply(vcg, auto)
-  by (meson CleanQ_RB_enq_y_inv_all CleanQ_RB_write_head_inv_all)
-
+  apply (meson CleanQ_RB_enq_y_inv_all CleanQ_RB_write_head_y_Invariant)
+  by (simp add: CleanQ_RB_enq_y_def CleanQ_RB_write_head_y_def)
 
 (* ------------------------------------------------------------------------------------ *)
 subsubsection \<open>Enqueue X, Dequeue X\<close>
@@ -1071,47 +1168,48 @@ subsubsection \<open>Enqueue X, Dequeue X\<close>
 paragraph \<open>Y reads the descriptor ring\<close>
 
 lemma CleanQ_CRB_Enqueue_X_P_read_tail:
-"\<Gamma>\<turnstile> \<lbrace> CleanQ_Enq_X_P K \<acute>RingCRB bx  \<rbrace> 
+"\<Gamma>\<turnstile> \<lbrace> CleanQ_RB_enq_x_P K \<acute>RingCRB bx  \<rbrace> 
      \<acute>b :== CleanQ_RB_read_tail_y \<acute>RingCRB 
-  \<lbrace>  CleanQ_Enq_X_P K \<acute>RingCRB bx  \<rbrace>"
+  \<lbrace>  CleanQ_RB_enq_x_P K \<acute>RingCRB bx  \<rbrace>"
   by(vcg)
 
 lemma CleanQ_CRB_Enqueue_X_Q_read_tail:
-"\<Gamma>\<turnstile> \<lbrace> CleanQ_Enq_X_Q K \<acute>RingCRB bx  \<rbrace> 
+"\<Gamma>\<turnstile> \<lbrace> CleanQ_RB_enq_x_Q K \<acute>RingCRB bx  \<rbrace> 
      \<acute>b :== CleanQ_RB_read_tail_y \<acute>RingCRB
-  \<lbrace>  CleanQ_Enq_X_Q K \<acute>RingCRB bx \<rbrace>"
+  \<lbrace>  CleanQ_RB_enq_x_Q K \<acute>RingCRB bx \<rbrace>"
   by(vcg)
 
 lemma CleanQ_CRB_Enqueue_X_R_read_tail:
-"\<Gamma>\<turnstile> \<lbrace> CleanQ_Enq_X_R K \<acute>RingCRB bx  \<rbrace> 
+"\<Gamma>\<turnstile> \<lbrace> CleanQ_RB_enq_x_R K \<acute>RingCRB bx  \<rbrace> 
      \<acute>b :== CleanQ_RB_read_tail_y \<acute>RingCRB
-  \<lbrace>  CleanQ_Enq_X_R K \<acute>RingCRB bx \<rbrace>"
+  \<lbrace>  CleanQ_RB_enq_x_R K \<acute>RingCRB bx \<rbrace>"
    by(vcg)
 
 paragraph \<open>Y increments the tail pointer\<close>
 
 lemma CleanQ_CRB_Enqueue_X_P_incr_tail:
-"\<Gamma>\<turnstile> \<lbrace>  b = CleanQ_RB_read_tail_y  \<acute>RingCRB \<and> b \<in> rSY \<acute>RingCRB \<and> CleanQ_RB_deq_y_possible \<acute>RingCRB \<and> CleanQ_Enq_X_P K \<acute>RingCRB bx  \<rbrace> 
+"\<Gamma>\<turnstile> \<lbrace>  b = CleanQ_RB_read_tail_y  \<acute>RingCRB \<and> b \<in> rSY \<acute>RingCRB \<and> CleanQ_RB_deq_y_possible \<acute>RingCRB \<and> CleanQ_RB_enq_x_P K \<acute>RingCRB bx  \<rbrace> 
       \<acute>RingCRB  :== CleanQ_RB_incr_tail_y b  \<acute>RingCRB 
-  \<lbrace>  CleanQ_Enq_X_P K \<acute>RingCRB bx  \<rbrace>"
+  \<lbrace>  CleanQ_RB_enq_x_P K \<acute>RingCRB bx  \<rbrace>"
   apply(vcg, auto simp:CleanQ_RB_deq_y_all_inv CleanQ_RB_deq_y_enq_x_possible )  
   using CleanQ_RB_deq_y_no_change by blast
 
 lemma CleanQ_CRB_Enqueue_X_Q_incr_tail:
-"\<Gamma>\<turnstile> \<lbrace>  b = CleanQ_RB_read_tail_y  \<acute>RingCRB \<and> b \<in> rSY \<acute>RingCRB \<and> CleanQ_RB_deq_y_possible \<acute>RingCRB \<and> CleanQ_Enq_X_Q K \<acute>RingCRB bx  \<rbrace> 
+"\<Gamma>\<turnstile> \<lbrace>  b = CleanQ_RB_read_tail_y  \<acute>RingCRB \<and> b \<in> rSY \<acute>RingCRB \<and> CleanQ_RB_deq_y_possible \<acute>RingCRB \<and> CleanQ_RB_enq_x_Q K \<acute>RingCRB bx  \<rbrace> 
      \<acute>RingCRB  :== CleanQ_RB_incr_tail_y b  \<acute>RingCRB 
-  \<lbrace>  CleanQ_Enq_X_Q K \<acute>RingCRB bx \<rbrace>"
+  \<lbrace>  CleanQ_RB_enq_x_Q K \<acute>RingCRB bx \<rbrace>"
   apply(vcg, auto simp:CleanQ_RB_deq_y_all_inv CleanQ_RB_deq_y_enq_x_possible ) 
   using CleanQ_RB_deq_y_no_change apply blast
-  by (metis CleanQ_RB_Invariants_def CleanQ_RB_deq_y_possible_def CleanQ_RB_read_tail_y_def
-            I2_rb_img_def I4_rb_valid_def disjoint_iff_not_equal hd_in_set prod.sel(1) 
-            rb_deq_def rb_deq_list_was_head rb_deq_not_empty rb_valid_def) 
+  apply (metis CleanQ_RB_Invariants_def CleanQ_RB_deq_y_possible_def CleanQ_RB_read_tail_y_def I2_rb_img_def I4_rb_valid_def IntI empty_iff prod.sel(1) rb_deq_def rb_deq_list_was_in)
+  by (metis CleanQ_RB_Invariants_def CleanQ_RB_deq_y_possible_def CleanQ_RB_read_tail_y_def I2_rb_img_def I4_rb_valid_def IntI empty_iff prod.sel(1) rb_deq_def rb_deq_list_was_in)
 
 lemma CleanQ_CRB_Enqueue_X_R_incr_tail:
-"\<Gamma>\<turnstile> \<lbrace>  b = CleanQ_RB_read_tail_y  \<acute>RingCRB \<and> b \<in> rSY \<acute>RingCRB \<and> CleanQ_RB_deq_y_possible \<acute>RingCRB \<and> CleanQ_Enq_X_R K \<acute>RingCRB bx  \<rbrace> 
+"\<Gamma>\<turnstile> \<lbrace>  b = CleanQ_RB_read_tail_y  \<acute>RingCRB \<and> b \<in> rSY \<acute>RingCRB \<and> CleanQ_RB_deq_y_possible \<acute>RingCRB \<and> CleanQ_RB_enq_x_R K \<acute>RingCRB bx  \<rbrace> 
      \<acute>RingCRB  :== CleanQ_RB_incr_tail_y b  \<acute>RingCRB 
-  \<lbrace>  CleanQ_Enq_X_R K \<acute>RingCRB bx \<rbrace>"
-  by(vcg, auto simp:CleanQ_RB_deq_y_all_inv CleanQ_RB_deq_y_enq_x_possible )
+  \<lbrace>  CleanQ_RB_enq_x_R K \<acute>RingCRB bx \<rbrace>"
+  apply(vcg, auto simp:CleanQ_RB_deq_y_all_inv CleanQ_RB_deq_y_enq_x_possible )
+  by (metis CleanQ_RB_Invariants_def CleanQ_RB_deq_y_possible_def CleanQ_RB_read_tail_y_def 
+            I2_rb_img_def I4_rb_valid_def IntI empty_iff prod.sel(1) rb_deq_def rb_deq_list_was_in)
 
 
 
@@ -1127,25 +1225,28 @@ lemma CleanQ_CRB_Dequeue_X_P_write_head:
 "\<Gamma>\<turnstile> \<lbrace> CleanQ_Deq_X_P K \<acute>RingCRB bx  \<rbrace> 
    \<acute>RingCRB :== CleanQ_RB_write_head_y b \<acute>RingCRB 
   \<lbrace>  CleanQ_Deq_X_P K \<acute>RingCRB bx  \<rbrace>"
-  apply(vcg, simp add:CleanQ_RB_enq_y_write_inv_all CleanQ_RB_write_head_y_can_enq_x[symmetric])
+  apply(vcg, auto)
+  apply (meson CleanQ_RB_write_head_y_Invariant)
   by (meson CleanQ_RB_write_head_y_can_deq_x)
 
 lemma CleanQ_CRB_Dequeue_X_Q_write_head:
 "\<Gamma>\<turnstile> \<lbrace> CleanQ_Deq_X_Q K \<acute>RingCRB bx  \<rbrace> 
    \<acute>RingCRB :== CleanQ_RB_write_head_y b \<acute>RingCRB 
   \<lbrace>  CleanQ_Deq_X_Q K \<acute>RingCRB bx \<rbrace>"
-  apply(vcg, simp add:CleanQ_RB_enq_y_write_inv_all CleanQ_RB_write_head_y_can_enq_x[symmetric]
+  apply(vcg, simp add: CleanQ_RB_write_head_y_can_enq_x[symmetric]
                       CleanQ_RB_write_head_y_can_deq_x[symmetric] )
-  apply(simp add: CleanQ_RB_read_tail_x_def CleanQ_RB_write_head_y_def )
-  by (metis CleanQ_RB_Invariants_def CleanQ_RB_deq_x_possible_def I4_rb_valid_def 
-            prod.sel(1) rb_deq_def rb_deq_list_was_head rb_enq_write_same rb_valid_def 
-            rb_write_can_deq rb_write_preserves_valid)
+  by (metis CleanQ_RB_Invariants_def CleanQ_RB_deq_x_possible_def CleanQ_RB_list_def 
+            CleanQ_RB_read_tail_x_def CleanQ_RB_write_head_y_I4 CleanQ_RB_write_head_y_Invariant 
+              CleanQ_RB_write_head_y_can_deq_x CleanQ_RB_write_head_y_list I4_rb_valid_def prod.sel(1) 
+              rb_deq_def rb_deq_list_was_head rb_read_tail_def rb_valid_implies_ptr_valid)
  
 lemma CleanQ_CRB_Dequeue_X_R_write_head:
 "\<Gamma>\<turnstile> \<lbrace> CleanQ_Deq_X_R K \<acute>RingCRB bx  \<rbrace> 
    \<acute>RingCRB :== CleanQ_RB_write_head_y b \<acute>RingCRB 
   \<lbrace>  CleanQ_Deq_X_R K \<acute>RingCRB bx \<rbrace>"
-  by(vcg, simp add:CleanQ_RB_enq_y_write_inv_all)  
+  apply(vcg)  
+  by (smt CleanQ_RB_write_head_y_Invariant Collect_cong hoarep.Basic mem_Collect_eq select_convs(1) 
+          surjective update_convs(1))
 
 paragraph \<open>Y increments the head pointer\<close>
 
@@ -1154,15 +1255,17 @@ lemma CleanQ_CRB_Dequeue_X_P_incr_head:
    \<acute>RingCRB :== CleanQ_RB_incr_head_y b rb 
   \<lbrace>  CleanQ_Deq_X_P K \<acute>RingCRB bx  \<rbrace>"
   apply(vcg, simp)
-  by (meson CleanQ_RB_enq_y_inv_all CleanQ_RB_write_head_inv_all  CleanQ_RB_enq_y_deq_x_possible CleanQ_RB_write_head_inv_all)
+  by (meson CleanQ_RB_enq_y_deq_x_possible CleanQ_RB_enq_y_inv_all CleanQ_RB_write_head_y_Invariant)
+  
+
   
 lemma CleanQ_CRB_Dequeue_X_Q_incr_head:
 "\<Gamma>\<turnstile> \<lbrace>  rb = CleanQ_RB_write_head_y b \<acute>RingCRB \<and> b \<in> rSY \<acute>RingCRB \<and> CleanQ_RB_enq_y_possible \<acute>RingCRB \<and> CleanQ_Deq_X_Q K rb bx  \<rbrace> 
    \<acute>RingCRB :== CleanQ_RB_incr_head_y b rb 
   \<lbrace>  CleanQ_Deq_X_Q K \<acute>RingCRB bx \<rbrace>"
   apply(vcg, auto) 
-  apply (meson CleanQ_RB_enq_y_inv_all CleanQ_RB_write_head_inv_all)
-  apply (meson CleanQ_RB_enq_y_deq_x_possible CleanQ_RB_write_head_inv_all) 
+  apply (meson CleanQ_RB_enq_y_inv_all CleanQ_RB_write_head_y_Invariant)
+  apply (meson CleanQ_RB_enq_y_deq_x_possible CleanQ_RB_write_head_y_Invariant)
   unfolding CleanQ_RB_read_tail_x_def CleanQ_RB_write_head_y_def CleanQ_RB_enq_y_def
   unfolding rb_read_tail_def rb_write_head_def rb_enq_def
   by (simp add: rb_incr_head_def)
@@ -1173,7 +1276,8 @@ lemma CleanQ_CRB_Dequeue_X_R_incr_head:
    \<acute>RingCRB :== CleanQ_RB_incr_head_y b rb 
   \<lbrace>  CleanQ_Deq_X_R K \<acute>RingCRB bx \<rbrace>"
   apply(vcg, auto)
-  by (meson CleanQ_RB_enq_y_inv_all CleanQ_RB_write_head_inv_all)
+  by (meson CleanQ_RB_enq_y_inv_all CleanQ_RB_write_head_y_Invariant)
+  
   
 
 
